src/Lexicographics.dfy
@@ -1,0 +1,95 @@
+// RUN: %dafny /compile:0 "%s"
+
+/*******************************************************************************
+*  Copyright by the contributors to the Dafny Project
+*  SPDX-License-Identifier: MIT 
+*******************************************************************************/
+
+include "Relations.dfy"
+
+module Lexicographics {
+    export 
+    reveals LexicographicByteSeqBelow, LexicographicByteSeqBelowAux 
+    provides Helpers, UInt, Relations
+
+    import Helpers = Relations.Helpers
+    import opened UInt = Helpers.UInt
+    import opened Relations
+
+  // reflexivelexicographical comparison of byte sequences
+  predicate method LexicographicByteSeqBelow(x: seq<uint8>, y: seq<uint8>) 
+  {
+    LexicographicByteSeqBelowAux(x, y, 0)
+  }
+
+  predicate method LexicographicByteSeqBelowAux(x: seq<uint8>, y: seq<uint8>, n: nat)
+    requires n <= |x| && n <= |y|
+    decreases |x| - n
+  {
+    || n == |x|
+    || (n != |y| && x[n] < y[n])
+    || (n != |y| && x[n] == y[n] && LexicographicByteSeqBelowAux(x, y, n + 1))
+  }
+
+  lemma AboutLexicographicByteSeqBelow()
+    ensures TotalOrdering(LexicographicByteSeqBelow)
+  {
+    assert Reflexive(LexicographicByteSeqBelow) by {
+      forall x, n | 0 <= n <= |x| {
+        AboutLexicographicByteSeqBelowAux_Reflexive(x, n);
+      }
+    }
+    assert AntiSymmetric(LexicographicByteSeqBelow) by {
+      forall x, y, n: nat |
+        n <= |x| && n <= |y| && x[..n] == y[..n] &&
+        LexicographicByteSeqBelowAux(x, y, n) && LexicographicByteSeqBelowAux(y, x, n)
+      {
+        AboutLexicographicByteSeqBelowAux_AntiSymmetric(x, y, n);
+      }
+    }
+    assert Helpers.Transitive(LexicographicByteSeqBelow) by {
+      forall x, y, z, n: nat |
+        n <= |x| && n <= |y| && n <= |z| &&
+        LexicographicByteSeqBelowAux(x, y, n) && LexicographicByteSeqBelowAux(y, z, n)
+      {
+        AboutLexicographicByteSeqBelowAux_Transitive(x, y, z, n);
+      }
+    }
+    assert Connected(LexicographicByteSeqBelow) by {
+      forall x, y, n: nat | n <= |x| && n <= |y| {
+        AboutLexicographicByteSeqBelowAux_Connected(x, y, n);
+      }
+    }
+  }
+
+  lemma AboutLexicographicByteSeqBelowAux_Reflexive(x: seq<uint8>, n: nat)
+    requires n <= |x|
+    ensures LexicographicByteSeqBelowAux(x, x, n)
+    decreases |x| - n
+  {
+  }
+
+  lemma AboutLexicographicByteSeqBelowAux_AntiSymmetric(x: seq<uint8>, y: seq<uint8>, n: nat)
+    requires n <= |x| && n <= |y|
+    requires x[..n] == y[..n]
+    requires LexicographicByteSeqBelowAux(x, y, n) && LexicographicByteSeqBelowAux(y, x, n)
+    ensures x == y
+    decreases |x| - n
+  {
+  }
+
+  lemma AboutLexicographicByteSeqBelowAux_Transitive(x: seq<uint8>, y: seq<uint8>, z: seq<uint8>, n: nat)
+    requires n <= |x| && n <= |y| && n <= |z|
+    requires LexicographicByteSeqBelowAux(x, y, n) && LexicographicByteSeqBelowAux(y, z, n)
+    ensures LexicographicByteSeqBelowAux(x, z, n)
+    decreases |x| - n
+  {
+  }
+
+  lemma AboutLexicographicByteSeqBelowAux_Connected(x: seq<uint8>, y: seq<uint8>, n: nat)
+    requires n <= |x| && n <= |y|
+    ensures LexicographicByteSeqBelowAux(x, y, n) || LexicographicByteSeqBelowAux(y, x, n)
+    decreases |x| - n
+  {
+  }
+}
